formalization/thesis/Isotope/LambdaIter/Subtyping/Named.lean
@@ -1,0 +1,3 @@
+import Isotope.LambdaIter.Subtyping.Named.Typing
+import Isotope.LambdaIter.Subtyping.Named.Structural
+import Isotope.LambdaIter.Subtyping.Named.Equiv
